doc/coq/simple/Bound.v
@@ -32,6 +32,28 @@ Definition time_bound_ρ `{TotalOrder T} (ρ : config T) :=
     time_bound_V V t /\ time_bound_m m t
   end.
 
+Ltac solve_leb1 :=
+  match goal with
+  | _ => assumption
+  | |- leb ?t ?t = true => apply leb_refl
+  | |- leb ?t (tick _ _ ?t _ _) = true => apply tick_lt
+  | |- leb _ (tick _ _ ?t _ _) = true => apply leb_trans with (t' := t)
+  | _ : leb ?a ?b = true |- leb ?a ?c = true => apply leb_trans with (t' := b)
+  | _ : supp_v ?v ?t |- _ => destruct v; ss
+  | H : time_bound_m ?m ?c, _ : supp_m ?m ?a |- leb ?a ?b = true =>
+    lazymatch b with
+    | c => apply H
+    | _ => apply leb_trans with (t' := b)
+    end
+  | H : time_bound_C ?C ?c, _ : supp_C ?C ?a |- leb ?a ?b = true =>
+    lazymatch b with
+    | c => apply H
+    | _ => apply leb_trans with (t' := b)
+    end
+  end.
+
+Ltac solve_leb := repeat solve_leb1.
+
 Lemma not_le_lt `{TotalOrder T} :
   forall (p : T) t,
     (leb p t = false) <-> (t << p).
@@ -121,7 +143,7 @@ Proof.
     subst. apply EQ. apply leb_sym; eauto.
 Qed.
 
-Lemma relax_mem_bound `{time T} :
+Lemma relax_mem_bound `{TotalOrder T} :
   forall m t1 t2 (BOUND : time_bound_m m t1) (LE : leb t1 t2 = true),
          time_bound_m m t2.
 Proof.
@@ -130,7 +152,7 @@ Proof.
   lebt t1. apply BOUND. eauto.
 Qed.
 
-Lemma time_bound_addr `{time T} :
+Lemma time_bound_addr `{TotalOrder T} :
   forall C x t (BOUND : time_bound_C C t),
     match addr_x C x with
     | None => True
@@ -154,30 +176,24 @@ Proof.
   end; apply BOUND; eauto.
 Qed.
 
-Lemma time_bound_read `{time T} :
+Lemma time_bound_read `{TotalOrder T} :
   forall m t addr (BOUND : time_bound_m m t),
     match read m addr with
     | None => True
-    | Some v => time_bound_v v t
+    | Some v => leb addr t = true /\ time_bound_v v t
     end.
 Proof.
   induction m; intros; simpl; eauto;
   repeat des_goal; repeat des_hyp; eauto;
   try rewrite eqb_eq in *; clarify;
-  match goal with
-  | _ => 
-    unfold time_bound_m in *;
-    unfold time_bound_v;
-    des_goal; red; intros; simpl in *;
-    apply BOUND; eauto; fail
-  | RR : read ?m ?addr = Some ?v |- _ => 
-    specialize (IHm t addr);
-    rewrite RR in IHm;
-    apply IHm; red; intros; apply BOUND; simpl; eauto
-  end.
+  unfold time_bound_m in *;
+  unfold time_bound_v in *.
+  - split; repeat des_goal; ii; apply BOUND; s; eauto.
+  - exploit (IHm t addr). ii. apply BOUND. s. eauto.
+    rw. eauto.
 Qed.
 
-Lemma time_bound_ctx_M `{time T} :
+Lemma time_bound_ctx_M `{TotalOrder T} :
   forall C M t (BOUND : time_bound_C C t),
     match ctx_M C M with
     | None => True
@@ -253,7 +269,7 @@ Proof.
     match goal with
     | H : time_bound_m m ?t |- _ =>
       pose proof (time_bound_read m t addr H);
-      rewrite RR in *; assumption
+      rewrite RR in *; des; assumption
     end
   | RR : ctx_M ?C ?M = Some _ |- _ =>
     let HINT := fresh "HINT" in
@@ -305,4 +321,166 @@ Proof.
     apply time_bound_tick; simpl; assumption]
   end;
   first [apply leb_refl | lebt t_a | lebt t'].
+Qed.
+
+Ltac gen_time_bound T :=
+  lazymatch goal with
+  | E1 : @step T _ _ _ (Cf ?e ?C ?m ?t) (Rs ?V ?m' ?t'),
+    E2 : {| (Cf ?e' ?C' ?m' ?t') ~> (Rs ?V' ?m'' ?t'') |},
+    E3 : {| (Cf ?e'' ?C'' ?m_up (tick ?C_v ?m'' ?t'' ?x ?v)) ~> (Rs ?V'' ?m''' ?t''') |} |- _ =>
+    let INC1 := fresh E1 in
+    let INC2 := fresh E2 in
+    let INC3 := fresh E3 in
+    apply time_increase in E1 as INC1;
+    apply time_increase in E2 as INC2;
+    apply time_increase in E3 as INC3;
+    let BD1 := fresh E1 in
+    apply time_bound in E1 as BD1;
+    lazymatch goal with
+    | _ : time_bound_ρ (Rs V m' t') |- _ =>
+      let BD2 := fresh E2 in
+      assert (time_bound_ρ (Cf e' C' m' t')) as BD2;
+      lazymatch goal with
+      | _ : time_bound_ρ (Cf e' C' m' t') |- _ =>
+        let BD2 := fresh E2 in
+        apply time_bound in E2 as BD2;
+        lazymatch goal with
+        | _ : time_bound_ρ (Rs V' m'' t'') |- _ =>
+          let BD3 := fresh E3 in
+          assert (time_bound_ρ (Cf e'' C'' m_up (tick C_v m'' t'' x v))) as BD3;
+          lazymatch goal with
+          | _ : time_bound_ρ (Cf e'' C'' m_up _) |- _ =>
+            let BD3 := fresh E3 in
+            apply time_bound in E3 as BD3;
+            try assumption
+          | _ => idtac
+          end
+        | _ => assumption
+        end
+      | _ => idtac
+      end
+    | _ => idtac
+    end
+  | E1 : @step T _ _ _ (Cf ?e ?C ?m ?t) (Rs ?V ?m' ?t'),
+    E2 : {| (Cf ?e' ?C' ?m' ?t') ~> (Rs ?V' ?m'' ?t'') |} |- _ =>
+    let INC1 := fresh E1 in
+    let INC2 := fresh E2 in
+    apply time_increase in E1 as INC1;
+    apply time_increase in E2 as INC2;
+    let BD1 := fresh E1 in
+    apply time_bound in E1 as BD1;
+    lazymatch goal with
+    | _ : time_bound_ρ (Rs V m' t') |- _ =>
+      let BD2 := fresh E2 in
+      assert (time_bound_ρ (Cf e' C' m' t')) as BD2;
+      lazymatch goal with
+      | _ : time_bound_ρ (Cf e' C' m' t') |- _ =>
+        let BD2 := fresh E2 in
+        apply time_bound in E2 as BD2;
+        try assumption
+      | _ => idtac
+      end
+    | _ => idtac
+    end
+  | E1 : @step T _ _ _ (Cf ?e ?C ?m ?t) (Rs ?V ?m' ?t'),
+    E2 : {| (Cf ?e' ?C' ?m_up (tick ?C_v ?m' ?t' ?x ?v)) ~> (Rs ?V' ?m'' ?t'') |} |- _ =>
+    let INC1 := fresh E1 in
+    let INC2 := fresh E2 in
+    apply time_increase in E1 as INC1;
+    apply time_increase in E2 as INC2;
+    let BD1 := fresh E1 in
+    apply time_bound in E1 as BD1;
+    lazymatch goal with
+    | _ : time_bound_ρ (Rs V m' t') |- _ =>
+      let BD2 := fresh E2 in
+      assert (time_bound_ρ (Cf e' C' m_up (tick C_v m' t' x v))) as BD2;
+      lazymatch goal with
+      | _ : time_bound_ρ (Cf e' C' m_up _) |- _ =>
+        let BD2 := fresh E2 in
+        apply time_bound in E2 as BD2;
+        try assumption
+      | _ => idtac
+      end
+    | _ => idtac
+    end
+  | E : @step T _ _ _ (Cf ?e ?C ?m ?t) (Rs ?V ?m' ?t') |- _ =>
+    let INC := fresh E in
+    apply time_increase in E as INC;
+    let BD := fresh E in
+    apply time_bound in E as BD; eauto
+  end;
+  lazymatch goal with
+  | |- time_bound_ρ _ =>
+    ss; des; split; red; ii; ss; des; clarify;
+    repeat match goal with
+    | |- leb ?t ?t = true => apply leb_refl
+    | |- leb _ (tick _ _ ?t _ _) = true => lebt t
+    | _ : supp_v ?v ?t |- _ => destruct v; ss
+    | H : time_bound_m ?m ?t'', _ : supp_m ?m ?t |- leb ?t ?t' = true =>
+      lazymatch t' with
+      | t'' => apply H; eauto
+      | _ => lebt t''
+      end
+    | H : time_bound_C ?C ?t'', _ : supp_C ?C ?t |- leb ?t ?t' = true =>
+      lazymatch t' with
+      | t'' => apply H; eauto
+      | _ => lebt t''
+      end
+    end
+  | _ => idtac
+  end.
+
+Lemma extend_mem `{time T} :
+  forall e C m t cf'
+         (EVAL : {|(Cf e C m t) ~> cf'|})
+         (BOUND : time_bound_ρ (Cf e C m t)),
+    match cf' with
+    | Rs _ m' _
+    | Cf _ _ m' _ =>
+      forall t' (LE : leb t' t = true),
+        read m' t' = read m t'
+    end.
+Proof.
+  intros.
+  remember (Cf e C m t) as cf.
+  ginduction EVAL; ii; des; clarify;
+  gen_time_bound T; s;
+  try match goal with
+  | |- (if eqb (tick ?C_v ?m_v ?t_v ?x ?v) ?t then _ else _) = read ?m ?t =>
+    ss; des; exploit (time_bound_read m _ t); eauto;
+    ii; des;
+    exploit (leb_t_neq_tick C_v m_v x v t t_v);
+    try (intros RR; rewrite eqb_comm in RR; rewrite RR; clear RR)
+  end;
+  solve_leb;
+  match goal with
+  | |- _ = read _ ?t =>
+    try (exploit IHEVAL3;
+      first [reflexivity 
+        | instantiate (1 := t); solve_leb
+        | solve [eauto] 
+        | ii; repeat rw; s]);
+    try (exploit IHEVAL2;
+      first [reflexivity 
+        | instantiate (1 := t); solve_leb 
+        | solve [eauto] 
+        | ii; repeat rw; s]);
+    try (exploit IHEVAL1;
+      first [reflexivity
+        | instantiate (1 := t); solve_leb  
+        | solve [eauto]
+        | ii; repeat rw; s]);
+    try (exploit IHEVAL;
+      first [reflexivity 
+        | instantiate (1 := t); solve_leb 
+        | solve [eauto]
+        | ii; repeat rw; s])
+  end;
+  try match goal with
+  | |- (if eqb (tick ?C_v ?m_v ?t_v ?x ?v) ?t then _ else _) = read ?m ?t =>
+    ss; des; exploit (time_bound_read m _ t); eauto;
+    ii; des;
+    exploit (leb_t_neq_tick C_v m_v x v t t_v);
+    try (intros RR; rewrite eqb_comm in RR; rewrite RR; clear RR)
+  end; solve [reflexivity | solve_leb].
 Qed.
