doc/coq/simple/Sound.v
@@ -13,30 +13,6 @@ Definition preserve_tick `{Concrete.time CT} `{Abstract.time AT} (α : CT -> AT)
   α (Concrete.tick C m t x v) = 
     Abstract.tick abs_C abs_m abs_t x abs_v.
 
-Ltac gen_leb :=
-  match goal with
-  | BD : time_bound_C ?C _, H : supp_C ?C _ |- _ =>
-    apply BD in H
-  | BD : time_bound_v ?v _, H : supp_v ?v _ |- _ =>
-    destruct v; unfold time_bound_v in BD; ss;
-    apply BD in H
-  | BD : time_bound_m ?m _, H : supp_m ?m _ |- _ =>
-    apply BD in H
-  | _ => idtac
-  end.
-
-Ltac solve_leb tac :=
-  match goal with
-  | _ => assumption
-  | |- leb ?t ?t = true => apply leb_refl
-  | _ : leb ?t ?t' = true |- leb ?t _ = true =>
-    lebt t';
-    match goal with
-    | _ : leb t' ?t'' = true |- _ => lebt t''
-    end
-  | _ => tac
-  end.
-
 Lemma trans_m_update `{TotalOrder T} {TT} (α : T -> TT) :
   forall m t t' v (BOUND : time_bound_m m t) (LT : t << t'),
     trans_m α (t' !-> v; m) =
@@ -115,23 +91,13 @@ Proof.
     pose proof (trans_C_ctx_M C α M);
     rewrite ACCESS in *; ss; eauto
   end;
-  repeat match goal with
-  | H : {| (Cf ?e ?C ?m ?t) ~> (Rs ?V ?m' ?t') |} |- _ =>
-    lazymatch goal with
-    | _ : leb t t' = true |- _ => fail
-    | _ =>
-      let INC := fresh "INC" in
-      let BD := fresh "BD" in
-      apply time_increase in H as INC;
-      first [solve [ss; eauto] | apply time_bound in H as BD]
-    end
-  end; ss; des;
+  gen_time_bound CT;
   try match goal with
   | |- {| _ ~#> _ |} =>
     try exploit IHEVAL1; eauto;
     try exploit IHEVAL2; eauto;
     try exploit IHEVAL3; eauto;
-    ii; ss; eauto (* simple cases are solved *)
+    ii; ss; des; eauto (* simple cases are solved *)
   end;
   (* difficult cases *)
   match goal with
@@ -141,21 +107,7 @@ Proof.
   | |- {| _ ~#> _ |} =>
     rewrite trans_m_update with (t := t') in *;
     first [apply tick_lt | rewrite PRES in *; eauto | assumption]
-  | |- _ /\ _ =>
-    try solve [split; eauto 3 using relax_ctx_bound]
-  | _ => idtac
-  end;
-  split; red; ii; ss; des; clarify;
-  gen_leb;
-  solve_leb ltac:(apply time_bound in EVAL2; ss; des);
-  match goal with
-  | |- _ /\ _ => solve [split; eauto 3 using relax_ctx_bound]
-  | |- _ /\ _ => split; red; ii; ss; des; clarify;
-    first [apply leb_refl | idtac]
-  | _ => idtac
-  end;
-  gen_leb;
-  solve_leb idtac.
+  end.
 Qed.
 
 (* soundness of linking *)
